\begin{alignat*}{5}
&\,&1+1\quad&=\quad&&2\\
&\,&\,&=\quad&&4-2\\
&\,&\,&=\quad&&4-\frac{9}{2}+\frac{9}{2}-2\\
&\,&\,&=\quad&&\sqrt{\left(4-\frac{9}{2}\right)^2}+\frac{9}{2}-2\\
&\,&\,&=\quad&&\sqrt{4^2-\cancel{2}(4)\left(\frac{9}{\cancel{2}}\right)+\left(\frac{9}{2}\right)^2}+\frac{9}{2}-2\\
&\,&\,&=\quad&&\sqrt{16-36+\left(\frac{9}{2}\right)^2}+\frac{9}{2}-2\\
&\,&\,&=\quad&&\sqrt{-20+\left(\frac{9}{2}\right)^2}+\frac{9}{2}-2\\
&\,&\,&=\quad&&\sqrt{25-45+\left(\frac{9}{2}\right)^2}+\frac{9}{2}-2\\
&\,&\,&=\quad&&\sqrt{25-2(5)\left(\frac{9}{2}\right)+\left(\frac{9}{2}\right)^2}+\frac{9}{2}-2\\
&\,&\,&=\quad&&\sqrt{5^2-2(5)\left(\frac{9}{2}\right)+\left(\frac{9}{2}\right)^2}+\frac{9}{2}-2\\
&\,&\,&=\quad&&\sqrt{\left(5-\frac{9}{2}\right)^2}+\frac{9}{2}-2\\
&\,&\,&=\quad&&5-\cancel{\frac{9}{2}}+\cancel{\frac{9}{2}}-2\\
&\small\text{Thus}\normalsize\qquad&1+1\quad&=\quad&&3
\end{alignat*}
