\begin{align*}
2+5\quad&\,=\quad4+3\\
\,&\,=\quad4-\frac{9}{2}+\frac{9}{2}+3\\
\,&\,=\quad\sqrt{\left(4-\frac{9}{2}\right)^2}+\frac{9}{2}+3\\
\,&\,=\quad\sqrt{16-2.4.\frac{9}{2}+\left(\frac{9}{2}\right)^2}+\frac{9}{2}+3\\
\,&\,=\quad\sqrt{16-36+\left(\frac{9}{2}\right)^2}+\frac{9}{2}+3\\
\,&\,=\quad\sqrt{-20+\left(\frac{9}{2}\right)^2}+\frac{9}{2}+3\\
\,&\,=\quad\sqrt{25-45+\left(\frac{9}{2}\right)^2}+\frac{9}{2}+3\\
\,&\,=\quad\sqrt{25-2.5.\frac{9}{2}+\left(\frac{9}{2}\right)^2}+\frac{9}{2}+3\\
\,&\,=\quad\sqrt{5^2-2.5.\frac{9}{2}+\left(\frac{9}{2}\right)^2}+\frac{9}{2}+3\\
\,&\,=\quad\sqrt{\left(5-\frac{9}{2}\right)^2}+\frac{9}{2}+3\\
\,&\,=\quad5-\cancel{\frac{9}{2}}+\cancel{\frac{9}{2}}+3\\
\mathrm{Thus}\qquad2+5\quad&\,=\quad8
\end{align*}
