\begin{alignat*}{5}
&\,&V_{ab}\quad&=\quad&&V_{an}\measuredangle0^\circ-V_{bn}\measuredangle120^\circ\\
&\,&\,&=&& V_{an}(\cos{0^\circ}+j\sin{{0^\circ}})-V_{bn}(\cos{120^\circ}+j\sin{{120^\circ}})\\
&\,&\,&=&&V_{an}(1+0)-V_{bn}(-\frac{1}{2}+j\cdot\frac{\sqrt{3}}{2})\\
&\,&V_{ab}\quad&=&&V_{an}-V_{bn}(-\frac{1}{2}+j\cdot\frac{\sqrt{3}}{2})\qquad&\small\text(1)\\
&\small\text{take magnitude}&|V_{an}|\quad&=&&|V_{bn}|\quad=\quad|V|\quad\small\text{(measure line to neutral)}\\
&\small\text{from (1)}&|V_{ab}|\quad&=&&|V|-|V|(-\frac{1}{2}+j\cdot\frac{\sqrt{3}}{2})\\
&\,&|V_{ab}|\quad&=&&|V|+\frac{1}{2}|V|-j|V|\cdot\frac{\sqrt{3}}{2}\\
&\,&\,&=&&|V|\frac{3}{2}-j|V|\cdot\frac{\sqrt{3}}{2}\\
&\,&\,&=&&|V|\left(\frac{3}{2}-j\cdot\frac{\sqrt{3}}{2}\right)\\
&\small\text{polar to rectangular}\normalsize\quad&|V_{ab}|\quad&=&&|V|\sqrt{\left(\frac{3}{2}\right)^2+\left(\frac{\sqrt{3}}{2}\right)^2}\\
&\,&\,&=&&|V|\sqrt{\frac{9}{4}+\frac{3}{4}}\\
&\,&\,&=&&|V|\sqrt{\frac{12}{4}}\\
&\qquad\qquad\small\text{Thus}\normalsize\qquad&|V_{ab}|\quad&=&&|V|\sqrt{3}\qquad\small\text{(valid proof)}\\
\end{alignat*}
