\begin{alignat*}{5}
&\,&6-7\quad&=\quad&&-1\\
&\,&\,&=&&2-3\\
&\,&\,&=&&2-\frac{5}{2}+\frac{5}{2}-3\\
&\,&\,&=&&\sqrt{\left(2-\frac{5}{2}\right)^2}+\frac{5}{2}-3\\
&\,&\,&=&&\sqrt{2^2-2(\cancel{2})\left(\frac{5}{\cancel{2}}\right)+\left(\frac{5}{2}\right)^2}+\frac{5}{2}-3\\
&\,&\,&=&&\sqrt{4-10+\left(\frac{5}{2}\right)^2}+\frac{5}{2}-3\\
&\,&\,&=&&\sqrt{-6+\left(\frac{5}{2}\right)^2}+\frac{5}{2}-3\\
&\,&\,&=&&\sqrt{9-15+\left(\frac{5}{2}\right)^2}+\frac{5}{2}-3\\
&\,&\,&=&&\sqrt{3^2-2(3)\left(\frac{5}{2}\right)+\left(\frac{5}{2}\right)^2}+\frac{5}{2}-3\\
&\,&\,&=&&\sqrt{\left(3-\frac{5}{2}\right)^2}+\frac{5}{2}-3\\
&\,&\,&=&&3-\frac{5}{2}+\frac{5}{2}-3\\
&\,&6-7\quad&=&&0\\
&\small\text{Thus}&6\quad&=&&7
\end{alignat*}
