\begin{align*}
\frac{-1}{1}\quad&\,=\quad\frac{1}{-1}\qquad(1)\\
\sqrt{\frac{-1}{1}}\quad&\,=\quad\sqrt{\frac{1}{-1}}\qquad(2)\\
\frac{\sqrt{-1}}{\sqrt{1}}\quad&\,=\quad\frac{\sqrt{1}}{\sqrt{-1}}\qquad(3)\\
\frac{i}{1}\quad&\,=\quad\frac{1}{i}\qquad(4)\\
*\,\frac{1}{2}\mathrm{~both~sides}\qquad\frac{i}{2}\quad&\,=\quad\frac{1}{2i}\qquad(5)\\
+\frac{3}{2i}\mathrm{~both~sides}\qquad\frac{i}{2}+\frac{3}{2i}\quad&\,=\quad\frac{1}{2i}+\frac{3}{2i}\qquad(6)\\
*~i\mathrm{~both~sides}\qquad i\left(\frac{i}{2}+\frac{3}{2i}\right)\quad&\,=\quad i\left(\frac{1}{2i}+\frac{3}{2i}\right)\qquad(7)\\
\frac{i^2}{2}+\frac{3\cancel{i}}{2\cancel{i}}\quad&\,=\quad\frac{\cancel{i}}{2\cancel{i}}+\frac{3\cancel{i}}{2\cancel{i}}\qquad(8)\\
-\frac{1}{2}+\frac{3}{2}\quad&\,=\quad\frac{1}{2}+\frac{3}{2}\qquad(9)\\
\frac{-1+3}{2}\quad&\,=\quad\frac{1+3}{2}\qquad(10)\\
\frac{\cancel{2}}{\cancel{2}}\quad&\,=\quad\cancelto{2}{\frac{4}{2}}\qquad(11)\\
1\quad&\,=\quad2\qquad(12)\\
\mathrm{from~(9)}\qquad-\frac{1}{2}+\cancel{\frac{3}{2}}\quad&\,=\quad\frac{1}{2}+\cancel{\frac{3}{2}}\qquad(13)\\
-\frac{1}{\cancel{2}}\quad&\,=\quad\frac{1}{\cancel{2}}\qquad(14)\\
-1\quad&\,=\quad1\qquad(15)\\
+1\mathrm{~both~sides}\qquad-1+1\quad&\,=\quad1+1\qquad(16)\\
0\quad&\,=\quad2\qquad(17)\\
\mathrm{from~(12),(15),(17)}\qquad-1~=~0~&\,=~1~=~2\qquad(18)
\end{align*}
