\begin{alignat*}{5}
&\,&e^x\quad&=\quad&&\sum_{i=0}^\infty\frac{x^n}{n!}\\
&\,&\,&=&&\frac{x^0}{0!}+\frac{x^1}{1!}+\frac{x^2}{2!}+\frac{x^3}{3!}+\frac{x^4}{4!}+...\\
&\,&e^x\quad&=&&1+\frac{x^1}{1}+\frac{x^2}{2!}+\frac{x^3}{3!}+\frac{x^4}{4!}+...\qquad&\small\text{(1)}\\
&\small\text{diff}&\frac{d}{dx}e^x\quad&=&&0+1+\frac{2x^1}{2!}+\frac{3x^2}{3!}+\frac{4x^3}{4!}+...\\
&\,&\,&=&&1+\frac{\cancel{2}x^1}{\cancel{2}.1!}+\frac{\cancel{3}x^2}{\cancel{3}.2!}+\frac{\cancel{4}x^3}{\cancel{4}.3!}+...\\
&\,&\,&=&&(1)\\
&\small\text{Thus}\normalsize\qquad&\frac{d}{dx}e^x\quad&=&&e^x\qquad\small\text{(valid proof)}
\end{alignat*}
