\begin{alignat*}{5}
&\,&&\qquad\quad e^{i\pi}\quad&&\,=\quad-1\\
&\text{power }i^3\text{ both sides}&&\qquad\left(e^{i\pi}\right)^{i^3}\quad&&\,=\quad-1^{i^3}\\
&\,&&\qquad\left(e^\pi\right)^{i^4}\quad&&\,=\quad\left(-1^{i^2}\right)^i\\
&\,&&\quad\left(e^\pi\right)^{i^2.i^2}\quad&&\,=\quad\left(-1^{-1}\right)^i\\
&\,&&\left(e^\pi\right)^{(-1)(-1)}\quad&&\,=\quad\left(\frac{1}{-1}\right)^i\\
&\,&&\qquad\left(e^\pi\right)^1\quad&&\,=\quad(-1)^i\\
&\text{power }2\text{ both sides}&&\qquad\quad e^{2\pi}\quad&&\,=\quad(-1)^{2i}\\
&\,&&\,&&\,=\quad1^i\\
&\text{from the previous proof}&&\,&&\,=\quad e^{-2\pi}\\
&\text{Thus}&&\qquad\quad e^{2\pi}&&\,=\quad e^{-2\pi}
\end{alignat*}
