\begin{alignat*}{5}
&\,&I^2\quad&=\quad&&\int_{-\infty}^\infty\,e^{-x^2}\,dx.\int_{-\infty}^\infty\,e^{-y^2}\,dy\\
&\,&\,&=&&\iint_{-\infty}^\infty\,e^{-(x^2+y^2)}\,dx\,dy\\
&\rlap{\small\text{convert the double integral into polar coordinates}}\\
&\,&I^2\quad&=&&\int_0^{2\pi}\int_0^\infty\,e^{-r^2}rdr\,d\theta\\
&\rlap{\small\text{the inner integral}}\\
&\,&\int_0^\infty\,e^{-r^2}rdr\quad&=&&\left.-\frac{1}{2}e^{-r^2}\right\vert_0^\infty\\
&\,&\,&=&&-\frac{1}{2}e^{-\infty^2}-\left(\frac{1}{2}e^{-0^2}\right)\\
&\,&\,&=&&-0-\left(-\frac{1}{2}\right)\\
&\,&\int_0^\infty\,e^{-r^2}rdr\quad&=&&\frac{1}{2}\\
&\rlap{\small\text{substituting this result back into the double integral}}\\
&\,&I^2\quad&=&&\int_0^{2\pi}\,\frac{1}{2}\,d\theta\\
&\,&\,&=&&\left.\frac{\theta}{2}\right\vert_0^{2\pi}\\
&\,&\,&=&&\frac{\cancel{2}\pi}{\cancel{2}}-\cancelto{0}{\frac{0}{2}}\\
&\,&I^2\quad&=&&\pi\\
&\,&\small\text{Thus}\normalsize\quad I~~\quad&=&&\sqrt{\pi}\quad\small\text{(valid proof)}
\end{alignat*}
