\begin{alignat*}{7}
&\,&\sin{x}&=&&\sum_{n=0}^{\infty}\frac{(-1)^n}{(2n+1)!}x^{2n+1}&=\quad&x-\frac{x^3}{3!}+\frac{x^5}{5!}-\frac{x^7}{7!}+\frac{x^9}{9!}-...\quad&\small\text{for all x}\\
&\,&\cos{x}&=&&\sum_{n=0}^{\infty}\frac{(-1)^n}{(2n)!}x^{2n}&=\quad&1-\frac{x^2}{2!}+\frac{x^4}{4!}-\frac{x^6}{6!}+\frac{x^8}{8!}-...\quad&\small\text{for all x}\\
&\,&e^x&=&&\sum_{n=0}^{\infty}\frac{x^n}{n!}&=\quad&1+x+\frac{x^2}{2!}+\frac{x^3}{3!}+\frac{x^4}{4!}+...\quad&\small\text{for all x}\\
&\,&e^{ix}&=&&\rlap{1+ix+\frac{(ix)^2}{2!}+\frac{(ix)^3}{3!}+\frac{(ix)^4}{4!}+ \frac{(ix)^5}{5!}+\frac{(ix)^6}{6!}+\frac{(ix)^7}{7!}+\frac{(ix)^8}{8!}+...}\\
&\,&\,&=\rlap{1+ix-\frac{x^2}{2!}-\frac{ix^3}{3!}+\frac{x^4}{4!}+\frac{ix^5}{5!}-\frac{x^6}{6!}-\frac{ix^7}{7!}+\frac{x^8}{8!}+...}\\
&\,&\,&=\rlap{\left(1-\frac{x^2}{2!}+\frac{x^4}{4!}-\frac{x^6}{6!}+\frac{x^8}{8!}-...\right)+i\left(x-\frac{x^3}{3!}+\frac{x^5}{5!}-\frac{x^7}{7!}+...\right)}\\
&\,&e^{ix}&=&&\cos{x}+i\sin{x}&\,&\small\text{***}\\
&\,&e^{ix}&=&&\cos{\pi}+\cancelto{0}{i\sin{\pi}}\\
&\small\text{Thus}&e^{i\pi}&=&&-1\quad\small\text{(valid proof)}
\end{alignat*}
