\begin{alignat*}{5}
&\,&&\quad e^x&&=\quad e^{i\pi.2\frac{x}{i\pi.2}}\\
&\,&&\,&&=\quad(e^{i\pi})^{2\frac{x}{2i\pi}}\\
&\,&&\,&&=\quad(-1)^{2\frac{x}{2i\pi}}\\
&\,&&\quad e^x&&=\quad1^\frac{x}{2i\pi}\qquad&&(1)\\
&\mathrm{as}\qquad&&\quad e^{i\pi}&&=\quad-1\\
&\,&&\ln{e^{i\pi}}&&=\quad\ln{(-1)}\\
&\,&&i\pi\cancelto{1}{\ln{e}}&&=\quad\ln{(-1)}\\
&\,&&\quad i\pi&&=\quad\ln{(-1)}\qquad&&(2)\\
&\mathrm{from~(1)}\qquad&&\quad e^x&&=\quad1^\frac{x}{2\ln(-1)}\\
&\,&&\,&&=\quad1^\frac{x}{\ln(-1^2)}\\
&\,&&\,&&=\quad1^\frac{x}{\cancelto{0}{\ln{1}}}\\
&\,&&\,&&=\quad1^\frac{x}{0}\\
&\,&&\,&&=\quad1^\infty\\
&\mathrm{Thus}\qquad&&\quad e^x&&=\quad1\qquad\mathrm{(so~foolish)}
\end{alignat*}
