\begin{alignat*}{7}
&\small\text{Let}\normalsize&x\quad&=\quad&&a\qquad&&\small\text{where }a{\text{ is any real number}}\\
&\,&x-a\quad&=&&0\\
&\,&(x-a)x\quad&=&&0\\
&\,&x^2-ax\quad&=&&0\\
&\,&x^2\quad&=&&ax\\
&\,&x\quad&=&&\sqrt{ax}&&\small\text{(1)}\\
&\small\text{substitue (1)}\normalsize&x\quad&=&&\sqrt{a\sqrt{ax}}\\
&\rlap{\small\text{indefinitely recursively substitute (1)}\normalsize}\\
&\,&x\quad&=&&\sqrt{a\sqrt{a\sqrt{a\sqrt{a\sqrt{\ldots}}}}}\\
&\small\text{since }x=a\text{, thus}\normalsize&x\quad&=&&\sqrt{x\sqrt{x\sqrt{x\sqrt{x\sqrt{\ldots}}}}}\qquad&&\small\text{(valid proof)}
\end{alignat*}
