\begin{alignat*}{5}
&\,&\infty^2\quad&=\quad&&\infty\qquad&\small\text{(1)}\\
&\,&\infty+1\quad&=&&\infty&\small\text{(2)}\\
&\small\text{(1)=(2)}\normalsize\quad&\infty^2\quad&=&&\infty+1\\
&\,&\infty^2-\infty-1\quad&=&&0\\
&\,&\infty\quad&=&&\frac{-(-1)\pm\sqrt{(-1^2)-4(1)(-1)}}{2(1)}\\
&\,&\,&=&&\frac{1\pm\sqrt{1+4}}{2}\\
&\small\text{take positive}&\infty\quad&=&&\frac{1+\sqrt{5}}{2}\\
&\,&\small\text{Thus}\normalsize\qquad\infty\quad&=&&\Phi\quad\small\text{a.k.a. Fibonacci golden ratio}
\end{alignat*}
