\begin{alignat*}{5}
&\,&-1\quad&=\quad&&e^{i\pi}\\
&\small\text{take ln both sides}&\ln{(-1)}\quad&=&&\ln{e^{i\pi}}\\
&\,&\,&=&&i\pi\cancelto{1}{\ln{e}}\\
&\,&\ln{(-1)}\quad&=&&i\pi&\small\text{(1)}\\
&\small\text{from (1)}&\sqrt{-\ln{(-1)}\ln{(-1)}}\quad&=&&\sqrt{-(i\pi)(i\pi)}\\
&\,&\,&=&&\sqrt{-(i\pi)^2}\\
&\,&\,&=&&\sqrt{-i^2\pi^2}\\
&\,&\,&=&&\sqrt{-(-1)(\pi^2)}\\
&\,&\,&=&&\sqrt{\pi^2}\\
&\small\text{Thus}&\sqrt{-\ln{(-1)}\ln{(-1)}}\quad&=&&\pi\qquad\small\text{(valid proof)}
\end{alignat*}
