\begin{alignat*}{7}
&\small{\text{Solve}}&x^3+x^2+x+1\quad&=\quad&&0&\small\text{(1)}\\
&\,&x^2+x+1\quad&=&&-x^3\qquad&\small\text{(2)}\\
&\small &divide x&x^2+x+1+\frac{1}{x}\quad&=&&0\\
&\small\text{from (2)}&\cancelto{-x^3}{(x^2+x+1)}+\frac{1}{x}\quad&=&&0\\
&\,&\frac{1}{x}\quad&=&&x^3\\
&\,&x^4\quad&=&&1&\small{(3)}\\
&\,&x\quad&=&&1\\
&\small\text{substitute (1)}\qquad&1^3+1^2+1+1\quad&=&&0\\
&\small\text{Thus}&4\quad&=&&0\\
&\rlap{\small\rm\underline{Caveat}\text{ solving (3) also results $x=\pm i\,\&-1$, which are the right solutions.}}\\
&\small\text{(1)}&x^3+x^2+x+1\quad&=\quad&&0\\
&\small x=i&-i-1+i+1\quad&=&&0\\
&\small x=-i\qquad&i-1-i+1\quad&=&&0\\
&\small x=-1&-1+1-1+1\quad&=&&0
\end{alignat*}
