\begin{alignat*}{5}
&\,&(n+1)^2\quad&=\quad&&n^2+2n+1\\
&\,&n^2\quad&=&&(n+1)^2-(2n+1)\\
&\small-n(2n+1)\text{ both sides}&n^2-n(2n+1)\quad&=&&(n+1)^2-(2n+1)-n(2n+1)\\
&\,&\,&=&&(n+1)^2-2n-1-2n^2-n\\
&\,&\,&=&&(n+1)^2-2n^2-3n-1\\
&\,&\,&=&&(n+1)^2-(2n^2+3n+1)\\
&\,&\,&=&&(n+1)^2-(n+1)(2n+1)\\
&\small+\frac{(2n+1)^2}{4}\text{ both sides}\normalsize\qquad&n^2-n(2n+1)+\frac{(2n+1)^2}{4}\quad&=&&(n+1)^2-(n+1)(2n+1)+\frac{(2n+1)^2}{4}\\
&\,&n^2-2n\frac{(2n+1)}{2}+\left(\frac{2n+1}{2}\right)^2\quad&=&&(n+1)^2-2(n+1)\left(\frac{2n+1}{2}\right)+\left(\frac{2n+1}{2}\right)^2\\
&\,&\left(n-\frac{2n+1}{2}\right)^2\quad&=&&\left((n+1)-\frac{2n+1}{2}\right)^2\\
&\small\sqrt{}\text{ both sides}&n-\cancel{\frac{2n+1}{2}}\quad&=&&n+1-\cancel{\frac{2n+1}{2}}\\
&\,&\small\text{Thus}\qquad\qquad\normalsize n\quad&=&&n+1
\end{alignat*}
