\begin{alignat*}{5}
&\,&e^{i\pi}\quad&=\quad&&-1\\
&\small\ln{}\text{ both sides}&\ln{e^{i\pi}}\quad&=&&\ln{(-1)}\\
&\,&i\pi\cancelto{1}{\ln{e}}\quad&=&&\ln{(-1)}\\
&\qquad\qquad\small\text{so}&\pi\quad&=&&\frac{\ln{(-1)}}{i}\qquad&\small\text{(1)}\\
&\small\times(-1)\text{ both sides}\qquad&-\pi\quad&=&&-\frac{\ln{(-1)}}{i}\\
&\,&\,&=&&\frac{\ln{(-1)}}{-i}\\
&\small\text{as }\frac{1}{-i}=i&\,&=&&i\ln{(-1)}\\
&\,&\,&=&&(-1)^{\frac{1}{2}}\ln{(-1)}\\
&\,&\,&=&&\left(\frac{1}{-1}\right)^\frac{1}{2}\ln{(-1)}\\
&\,&\,&=&&\frac{1^\frac{1}{2}}{(-1)^\frac{1}{2}}\ln{(-1)}\\
&\,&\,&=&&\frac{1}{\sqrt{-1}}\ln{(-1)}\\
&\,&\,&=&&\frac{1}{i}\ln{(-1)}\\
&\qquad\qquad\small\text{so}&-\pi\quad&=&&\frac{\ln{(-1)}}{i}\qquad&\small\text{(2)}\\
&\qquad\qquad\small\text{hence}&(1)\quad&=&&(2)\\
&\qquad\qquad\small\text{Thus}&\pi\quad&=&&-\pi
\end{alignat*}
