\begin{alignat*}{4}
&\,&&\qquad e^{i\pi}&&\,=\qquad-1\\
&\,&&\qquad (e^{i\pi})^2&&\,=\qquad(-1)^2\\
&\,&&\qquad e^{2i\pi}&&\,=\qquad1&&\qquad(1)\\
&\,&&\qquad e^{2i\pi}.e&&\,=\qquad e\\
&\,&&\qquad e^{2i\pi+1}&&\,=\qquad e\\
&\,&&\left(e^{2i\pi+1}\right)^{2i\pi+1}&&\,=\qquad e^{2i\pi+1}\\
&\,&&e^{(2i\pi+1)(2i\pi+1)}&&\,=\qquad e^{2i\pi}.e\\
&\mathrm{from~(1)}\qquad&&e^{(2i\pi+1)(2i\pi+1)}&&\,=\qquad1e\\
&\,&&e^{(2i\pi)^2+2.2i\pi+1^2}&&\,=\qquad e\\
&\,&&e^{(-4\pi^2+4i\pi+1)}&&\,=\qquad e\\
&\,&&e^{-4\pi^2}.e^{4i\pi}.\cancel{e}&&\,=\qquad\cancel{e}\\
&\,&&e^{-4\pi^2}.e^{4i\pi}&&\,=\qquad1\\
&\,&&e^{-4\pi^2}.e^{i\pi.2.2}&&\,=\qquad1\\
&\,&&e^{-4\pi^2}.(-1)^{2.2}&&\,=\qquad1\\
&\,&&\quad e^{-4\pi^2}.\cancel{1}^2&&\,=\qquad\cancel{1}\\
&\,&&\quad \ln{(e^{-4\pi^2})}&&\,=\qquad\ln1\\
&\,&&-4\pi^2\cancelto{1}{\ln{(e)}}&&\,=\qquad0\\
&\,&&\qquad \pi^2&&\,=\qquad0\\
&\mathrm{Thus}&&\qquad \pi&&\,=\qquad0
\end{alignat*}
