\begin{alignat*}{5}
&\qquad\small\text{Let}&x\quad&=\quad&&\frac{\pi+e}{2}\\
&\small\times2&2x\quad&=&&\cancel{2}\cdot\frac{\pi+e}{\cancel{2}}\\
&\small\times(\pi-e)\qquad&2x(\pi-e)\quad&=&&(\pi+e)(\pi-e)\\
&\,&2\pi x-2ex\quad&=&&\pi^2-e^2\\
&\,&-\pi^2+2\pi x\quad&=&&-e^2+2ex\\
&\small\times-1&\pi^2-2\pi x\quad&=&&e^2-2ex\\
&\small+x^2&\pi^2-2\pi x+x^2\quad&=&&e^2-2ex+x^2\\
&\,&\left(\pi-x\right)^2\quad&=&&(e-x)^2\\
&\,&\pi-\cancel{x}\quad&=&&e-\cancel{x}\\
&\qquad\small\text{Thus}&\pi\quad&=&&e
\end{alignat*}
