\begin{alignat*}{5}
&\small\text{from the previous proof}&-1\quad&=\quad&&1\qquad\quad&\small\text{(1)}\\
&\,&\ln{(-1)}\quad&=&&\ln{(1)}\\
&\,&\ln{e^{i\pi}}\quad&=&&0\\
&\,&i\pi\cancelto{1}{\ln{e}}\quad&=&&0\\
&\,&i\pi\quad&=&&0\\
&\small\times2i\text{ both sides}&2i\cdot\,i\pi\quad&=&&2i\cdot\,0\\
&\,&2i^2\pi\quad&=&&0\\
&\small\,i^2=-1&-2\pi\quad&=&&0&\small\text{(2)}\\
&\small\text{(1)}\times\text{(2)}&2\pi\quad&=&&0&\small\text{(3)}\\
&\qquad\qquad\small\text{Thus}&\pm2\pi\quad&=&&0
\end{alignat*}
