\begin{align*}
S\quad&\,=\quad1+2+3+...\\
\mathrm{Let}\qquad S_1\quad&\,=\quad1-1+1-1+...\\
1-S_1\quad&\,=\quad1-(1+1-1+1-...)\\
1-S_1\quad&\,=\quad1-1+1-1+...\\
1-S_1\quad&\,=\quad S1\\
2S_1\quad&\,=\quad1\\
S_1\quad&\,=\quad\frac{1}{2}\\
\mathrm{Let}\qquad S_2\quad&\,=\quad1-2+3-4+5-6+...\\
2S_2\quad&=\quad1-2+3-4+5-6+...\\
\quad&\,\qquad\quad\,+1-1+3-4+5-6\\
2S_2\quad&\,=\quad1-1+1-1+...\\
2S_2\quad&\,=\quad S_1\\
S_2\quad&\,=\quad\frac{S_1}{2}\\
S_2\quad&\,=\quad\frac{1}{4}\\
S-S_2\quad&\,=\quad1+2+3+4+5+6+7+8+...\\
\quad&\,\quad-(1-2+3-4+5-6+7-...)\\
S-S_2\quad&\,=\quad4+8+12+16+...\\
S-S_2\quad&\,=\quad4(1+2+3+4+...)\\
S-S_2\quad&\,=\quad4S\\
3S\quad&\,=\quad-S_2\\
S\quad&\,=\quad-\frac{S_2}{3}\\
S\quad&\,=\quad-\frac{1}{3*4}\\
\mathrm{Thus}\qquad S\quad&\,=\quad-\frac{1}{12}
\end{align*}
