\begin{alignat*}{5}
&\,&-1\quad&=\quad&&e^{i\pi}\\
&\small\text{power }\normalsize i^3&\left(-1\right)^{i^3}\quad&=&&(e^{i\pi})^{i^3}\\
&\,&-1^{i^2i}\quad&=&&e^{i^4\pi}\\
&\,&-1^{-1i}\quad&=&&e^{(i^2)^2\pi}\\
&\,&-1^{-i}\quad&=&&e^{-1^2\pi}\\
&\,&-1^{-i}\quad&=&&e^{1\pi}\\
&\small\text{as }\normalsize -i=\frac{1}{i}&-1^\frac{1}{i}\quad&=&&e^\pi\\
&\small\text{power }\normalsize 2&-1^\frac{2}{i}\quad&=&&e^{2\pi}\\
&\,&\left(-1^2\right)^\frac{1}{i}\quad&=&&e^{2\pi}\\
&\,&\quad1^{\frac{1}{i}}\quad&=&&e^{2\pi}\\
&\qquad\small\text{Thus}&\sqrt[^i]{1}\quad&=&&e^{2\pi}
\end{alignat*}
